Continue sketching egraph work

src/Utils/Monad.v
@@ -1,16 +1,21 @@
 Set Implicit Arguments.
 Set Bullet Behavior "Strict Subproofs".
 
+Require List.
+
 Class Monad (M : Type -> Type) : Type :=
   {
   Mret : forall {A}, A -> M A;
   Mbind : forall {A B}, (A -> M B) -> M A -> M B
   }.
 
+Definition Mseq {M} `{Monad M} {A B} (mu : M A) (ma : M B) : M B :=
+  Mbind (fun _ => ma) mu.
 
 Declare Custom Entry monadic_do.
 
-Notation "'do' e" := (e) (at level 200, e custom monadic_do).
+(* I would use 'do', but it interferes with proof general indentation *)
+Notation "@! e" := (e) (at level 200, e custom monadic_do).
 
 
 Notation "'let' p <- e 'in' b" :=
@@ -35,6 +40,12 @@ Notation "'if' c 'then' b1 'else' b2" :=
     (in custom monadic_do at level 200, left associativity,
         c constr, b1 custom monadic_do, b2 custom monadic_do).
 
+Notation "e1 ; e2" :=
+  (Mseq e1 e2)
+    (in custom monadic_do at level 100, left associativity,
+        e1 custom monadic_do,
+        e2 custom monadic_do).
+
 Notation "'ret' e" := (Mret e) (in custom monadic_do at level 90, e constr).
 
 Notation "e" := e (in custom monadic_do at level 90, e constr at level 0).
@@ -50,4 +61,95 @@ TODO: add fail
 
 Generalizable Variable M.
 Definition Mfmap `{mmon:Monad M} {A B:Set} (f : A -> B) (ma: M A) : M B :=
-  do let a <- ma in ret f a.
+  @! let a <- ma in ret f a.
+
+(*TODO: move these into separate files? *)
+
+Section MonadListOps.
+  Import List List.ListNotations.
+  Context {M A B} `{Monad M}
+          (f : A -> M B).
+
+  Fixpoint list_Mmap (l : list A) : M (list B) :=
+    match l with
+    | [] => @! ret []
+    | a::al' =>
+        @! let b <- f a in
+           let bl' <- list_Mmap al' in
+           ret (b::bl')
+    end.
+  
+  Fixpoint list_Miter (f : A -> M unit) (l : list A) : M unit :=
+    match l with
+    | [] => @! ret tt
+    | a::al' =>
+        @! let b <- f a in
+           let tt <- list_Miter f al' in
+           ret tt
+    end.
+End MonadListOps.
+
+
+From coqutil Require Map.Interface.
+
+Module StateMonad.
+
+  Definition ST S A := S -> (S * A).
+
+  Instance state_monad {S} : Monad (ST S) :=
+    {
+      Mret _ a := fun s => (s,a);
+      Mbind _ _ f ma :=
+      fun s =>
+        let (s,a) := ma s in
+        f a s
+    }.
+
+  
+  (*TODO: double check this is the right name*)
+  (* backtracks the state if ma returns None *)       
+  Definition try_with_backtrack {S A}
+             (ma : ST S (option A)) : ST S (option A) :=
+    fun g =>
+      match ma g with
+      | (g', Some a) => (g', Some a)
+      | (_, None) => (g, None)
+      end.
+  
+  Section MapOps.
+    
+    Import Map.Interface.
+    
+    Definition map_Mfold {S K V A}
+               {MP : map.map K V}
+               (f : K -> V -> A -> ST S A)
+               (p : @map.rep _ _ MP) a : ST S A :=
+      fun g =>
+        map.fold
+          (fun '(g, a) k v => f k v a g)
+          (g, a) p.
+
+    Definition map_Miter {S K V}
+               {MP : map.map K V}
+               (f : K -> V -> ST S unit)
+               (p : @map.rep _ _ MP) : ST S unit :=
+      map_Mfold (fun k v _ => f k v) p tt.
+
+  End MapOps.
+
+  Notation "'for' kp vp 'from' m 'in' b" :=
+    (map_Miter (fun kp vp => b) m)                       
+      (in custom monadic_do at level 200, left associativity,
+          kp pattern at level 0,
+          vp pattern at level 0,
+          m constr, b custom monadic_do).
+  
+  Notation "'for/fold' kp vp 'from' m [[ acc := a ]] 'in' b" :=
+    (map_Mfold (fun kp vp acc => b) a m)                       
+      (in custom monadic_do at level 200, left associativity,
+          kp pattern at level 0,
+          vp pattern at level 0,
+          acc pattern at level 0,
+          m constr, b custom monadic_do).
+
+End StateMonad.
