src/named/egraph/Defs.v
@@ -4,670 +4,533 @@
 Set Implicit Arguments.
 Set Bullet Behavior "Strict Subproofs".
 
-Require Import Bool String List Orders ZArith.
+Require Import Bool String List ZArith.
 Import ListNotations.
 Open Scope string.
 Open Scope list.
-(*TODO: link coqutil
 From coqutil Require Import Map.Interface.
-From coqutil Require Map.SortedList.*)
-From Utils Require Import Utils PersistentArrayList UnionFind Natlike.
-From Named Require Import Term.
+From Utils Require Import Utils Natlike ExtraMaps Monad RelationalDB.
+Import Sets.
+From Utils Require ArrayList UnionFind.
+From Named Require Import Term Rule.
 (*Import Core.Notations.*)
 
-Require MSets.
+(*TODO: move to utils*)
+Definition unwrap_with_default {A} (default : A) ma :=
+  match ma with None => default | Some a => a end.
 
-(*TODO: eqb from natlike *)
-#[refine]
- Instance eqb_natlike A `{Ops.NatlikeOps A} : Eqb A :=
-  {|
-    eqb := Ops.eqb
-  |}.
-Proof.
-Admitted.
-    
+Section __.
+  Context {idx : Type}
+          `{Natlike idx}
+          {array : Type -> Type}
+          `{ArrayList.ArrayList idx array}.
+  
+  Notation named_list := (@named_list idx).
+  Notation named_map := (@named_map idx).
+  Notation term := (@term idx).
+  Notation ctx := (@ctx idx).
+  Notation sort := (@sort idx).
+  Notation subst := (@subst idx).
+  Notation rule := (@rule idx).
+  Notation lang := (@lang idx).
 
+  Notation union_find := (@UnionFind.union_find idx array).
+  
+  Variant enode :=
+    (* CONVENTION: for terms, first element of args is the sort *)
+    (* TODO: determine if this is a good way to do it *)
+    | con_node : idx -> list idx -> enode
+    (*TODO: separate constructor for sorts?  | scon_node : list idx -> enode *)
+    | var_node : (*(* sort id*) idx ->*) (* var *) idx -> enode.
 
-(*TODO: parameterize by ArrayList impl;
-  depends on UnionFind coq bug
- *)
-Import Int63.
-Import OrdersEx.
-
-(*TODO: move anything not touching terms or nodes to utils, nodes to sep. file*)
-
-(*TODO: is this defined anywhere?*)
-Module ListDecidableType(D :DecidableType) <: DecidableType.
-
-  Definition t := list D.t.
-
-  Definition eq := Forall2 D.eq.
-
-  #[global]
-   Instance eq_equiv : Equivalence eq.
-  Proof.
-    unfold eq.
-    repeat constructor.
-    {
-      intro l; induction l;
-        constructor; eauto.
-      apply D.eq_equiv.
-    }
-    {
-      intro l; induction l;
-      inversion 1;
-      constructor; eauto;
-      subst.
-      apply D.eq_equiv; auto.
-    }
-    {
-      intro l; induction l;
-      inversion 1;
-      inversion 1;
-      subst;
-      constructor; eauto.
-      destruct D.eq_equiv as [_ _ Dtrans];
-        eapply Dtrans; eauto.
-    }
-  Qed.  
-
- Definition eq_dec : forall x y, { eq x y }+{ ~eq x y }.
- Proof.
-   unfold eq.
-   induction x; destruct y; eauto.
-   1,2: right; inversion 1.
-   destruct (D.eq_dec a t0);
-     destruct (IHx y).
-   {
-     intuition.
-   }
-   all: right; inversion 1; subst; auto.
- Defined.
- 
-End ListDecidableType.
-
-Module ListOrderedType(O:OrderedType) <: OrderedType.
-  Include ListDecidableType O.
-
-  Definition lt : t -> t -> Prop. Admitted.
-
-  #[global]
-   Instance lt_strorder : StrictOrder lt.
-  Proof.
-  Admitted.
-
-  #[global]
-   Instance lt_compat : Proper (eq==>eq==>iff) lt.
-  Proof.
-  Admitted.
-
-  Fixpoint compare x y :=
-    match x, y with
-    | [], [] => Eq
-    | [], _ => Lt
-    | _, [] => Gt
-    | (a::x), (b::y) =>
-      match O.compare a b with
-      | Eq => compare x y
-      | Lt => Lt
-      | Gt => Gt
-      end
-    end.
-
- Lemma compare_spec : forall x y, CompSpec eq lt x y (compare x y).
- Proof.
- Admitted.
-
-End ListOrderedType.
-
-Fixpoint list_ltb {A} (ltb : A -> A -> bool) (a b : list A) : bool :=
-    match a,b with
-    | [], [] => false
-    | [], _ => true
-    | _, [] => false
-    | (a::x), (b::y) =>
-      (ltb a b) && (list_ltb ltb x y)
-    end.
-
-Module IntListOT := ListOrderedType Int63Natlike.
-
-(*Define aliases for int so that at least the type annotations are more descriptive*)
-Definition var_idx := int.
-Definition constr_idx := int.
-Definition srt_idx := int.
-Definition ctx_idx := int.
-Definition tm_idx := int.
-
-(*TODO: use string -> int mapping to convert lang, ctx so that the egraph
-  does not store strings
-*)
-Variant enode :=
-(*TODO: look into efficient ways to optimize empty if looking for a little performance(null?)*)
-| ctx_empty_node : enode
-| ctx_cons_node : (*context length*) N -> var_idx -> srt_idx -> ctx_idx -> enode
-| con_node : constr_idx ->  list tm_idx -> enode
-| scon_node : constr_idx -> list tm_idx -> enode
-| var_node : var_idx -> enode.
+  Context {node_set : set enode}
+          {node_map : map.map enode idx}.
 
 
-Axiom TODO: forall {A}, A.
-Module ENode <: OrderedType.
-  (*TODO: have separate scon node or optional type?*)
-
-  Definition t := enode.
-
-  (*TODO
-  Definition eq n1 n2 :=
-    match n1, n2 with
-    | ctx_empty_node, ctx_empty_node => true
-    | ctx_cons_node var1 srt1 tl1, ctx_cons_node var2 srt2 tl2 => 
-    | con_node : string -> (*ctx *) int -> (*sort*) int -> list int -> enode
-    | acon_node : string -> (*ctx *) int -> list int -> enode
-    | var_node : string -> (*ctx *) int -> (*sort*) int -> enode.
-      
-
-  Definition ltb '(n1, args1) '(n2,args2) :=
-    (String.ltb n1 n2) && (list_ltb Int63.ltb args1 args2).
+  (* TODO : separate sort eclasses? it would avoid awkwardness around esort dummy value
    *)
+  Record eclass : Type :=
+    MkEClass {
+        nodes : node_set;
+        parents : node_map;
+        (* value is unused if the class represents a sort
+         TODO: is this the best way? could also fix it as 0
+        
+        esort : idx;*)
+      }.
 
-  Definition eq := @eq t.
-  Definition eq_equiv : Equivalence eq := TODO.
-  Definition lt : t -> t -> Prop := TODO.
+  Context {eclass_map : map.map idx eclass}.
+  (*{idx_map : map.map idx idx}*)
 
-  #[global]
-   Instance lt_strorder : StrictOrder lt.
-  Proof.
-  Admitted.
+  (* Fix a specific context that the egraph is operating in.
+     This means that we can't reuse egraphs between rules
+     in a proof of compiler correctness,
+     but it is difficult to do so even when tracking multiple contexts.
 
-  #[global]
-   Instance lt_compat : Proper (eq==>eq==>iff) lt.
-  Proof.
-  Admitted.
-
-  Definition compare : t -> t -> comparison := TODO.
-
-  Lemma compare_spec : forall x y, CompSpec eq lt x y (compare x y).
-  Proof.
-  Admitted.
-  
-  Definition eq_dec : forall x y, { eq x y }+{ ~eq x y }.
-  Proof.
-  Admitted.
-
-  Definition ltb : t -> t -> bool.
-  Admitted.
-    
-End ENode.
-
-
-Module NodeSets := MSets.MSetAVL.Make ENode.
-
-(*
-Module Parents := PairOrderedType ENode Int63Natlike.
-Module ParentSets := MSets.MSetAVL.Make Parents.
-*)
-
-
-Module Int63Map.
-  (* Make this an instance so we can use single-curly-braces so we don't need to qualify field-names with [SortedList.parameters.] *)
-  Import Int63Natlike.
-  Local Instance int63_strict_order: @SortedList.parameters.strict_order _ ltb.
-  {
-    constructor.
-    {
-      intros.
-      rewrite <- not_true_iff_false.
-      rewrite ltb_lt.
-      int_lia.
-    }
-    {
-      intros.
-      rewrite ltb_lt in *.
-      int_lia.
-    }
-    {
-      intros.
-      rewrite <- not_true_iff_false in *.
-      rewrite ltb_lt in *.
-      int_lia.
-    }
-  }
-  Qed.
-  
-  Definition Build_parameters T :=
-    SortedList.parameters.Build_parameters _ T ltb.
-  
-  Definition map T := SortedList.map (Build_parameters T) int63_strict_order.
-
-  Definition ok T : @Interface.map.ok _ T (map T).
-    pose proof @SortedList.map_ok (Build_parameters T) as H; eapply H.
-  Qed.
-  
-End Int63Map.
-
-
-  (*TODO: representation choice: each eclass should only need a single sort, ctx
-    currently, each enode has them.
-    Fix?
-    Related: Do I want one eclass per context for closed terms like 'true'?
-    or one eclass for all things equal to 'true'?
-    The latter doesn't seem sound, but the former might be a bit expensive
-    Related: how to work w/ meta-level substitutions in egraphs?
-
-    Optimal solution prob. involves special treatment/eqns for metavar substs
+     On user programs this is generally the empty context.
    *)
+  Record egraph :=
+    MkEGraph {
+        (* TODO: context sorts added to the egraph at initialization *)
+        ectx : named_list idx;
+        id_equiv : union_find;
+        eclasses : eclass_map;
+        hashcons : node_map;
+        worklist : list idx
+      }.
 
-Module ENodeMap.
-  (* Make this an instance so we can use single-curly-braces so we don't need to qualify field-names with [SortedList.parameters.] *)
-  Import ENode.
-  Local Instance enode_strict_order: @SortedList.parameters.strict_order _ ENode.ltb.
-  Admitted (*TODO: use existing strorder?*).
-  
-  Definition Build_parameters T :=
-    SortedList.parameters.Build_parameters _ T ltb.
-  
-  Definition map T := SortedList.map (Build_parameters T) enode_strict_order.
-
-  Definition ok T : @Interface.map.ok _ T (map T).
-    pose proof @SortedList.map_ok (Build_parameters T) as H; eapply H.
-  Qed.
-  
-End ENodeMap.
-
-Instance hashcons_ty : Interface.map.map ENode.t Int63Natlike.t := ENodeMap.map _.
-
-(* TODO : could split off ctx classes here or even further (a separate pool)
-   since they behave differently (no direct eqns, only unified as parents of subterms).
-   Think about efficiency
-*)
-Record eclass : Type :=
-  MkEClass {
-      nodes : NodeSets.t;
-      parents : ENodeMap.map Int63Natlike.t;
-      (* value is unused if the class represents a ctx
-         TODO: is this the best way?
-       *)
-      ectx : int;
-      (* value is unused if the class represents a ctx or sort
-         TODO: is this the best way?
-       *)
-      esrt : int;
-    }.
-
-Module EClass.
-
-  (* Include a parent map in each eclass *)
-  Definition t : Type := eclass.
 
   (*Definition union '(ns1,ps1) '(ns2,ps2) : t :=
     (NodeSets.union ns1 ns2, (*TODO: need map union?*)map.union ps1 ps2).*)
 
-  Definition empty ctx srt : t :=
-    MkEClass NodeSets.empty map.empty ctx srt.
+  Definition eclass_empty : eclass :=
+    MkEClass map.empty map.empty.
 
+  (* more common to call than empty *)
   (* Assumes no parents *)
-  Definition singleton n ctx srt : t := 
-    MkEClass (NodeSets.singleton n) map.empty ctx srt.
+  Definition eclass_singleton n : eclass := 
+    MkEClass (map.singleton n tt) map.empty.
 
-  Definition add_parent '(MkEClass ns ps ntx nsrt) '(pn,pi) : t :=
-    MkEClass ns (map.put ps pn pi) ntx nsrt.
+  Definition eclass_add_parent '(MkEClass ns ps) '(pn,pi) : eclass :=
+    MkEClass ns (map.put ps pn pi).
   
-End EClass.
-
-
-Instance eclass_map_ty : Interface.map.map Int63Natlike.t EClass.t := Int63Map.map _.
-
-Module UF := CBVUnionFind.
-
-Record egraph :=
-  MkEGraph {
-      id_equiv : UF.M.union_find;
-      eclass_map : Int63Map.map EClass.t;
-      hashcons : ENodeMap.map Int63Natlike.t;
-      worklist : list Int63Natlike.t
-  }.
-
-Require Import Utils.Monad.
-
-Definition ST S A := S -> (S * A).
-
-Instance state_monad {S} : Monad (ST S) :=
-  {
-  Mret _ a := fun s => (s,a);
-  Mbind _ _ f ma :=
-    fun s =>
-      let (s,a) := ma s in
-      f a s
-  }.
-
-Section MonadListMap.
-  Context {M A B} `{Monad M}
-          (f : A -> M B).
-
-  Fixpoint list_Mmap (l : list A) : M (list B) :=
-    match l with
-    | [] => do ret []
-             | a::al' =>
-               do let b <- f a in
-                  let bl' <- list_Mmap al' in
-                  ret (b::bl')
-                  end.
-End MonadListMap.
-       
-Fixpoint list_Miter {M A} `{Monad M} (f : A -> M unit) (l : list A) : M unit :=
-  match l with
-  | [] => do ret tt
-  | a::al' =>
-    do let b <- f a in
-       let tt <- list_Miter f al' in
-       ret tt
-       end.
-
-Definition unwrap_with_default {A} (default : A) ma :=
-  match ma with None => default | Some a => a end.
-
-
-Definition map_Mfold {S K V A}
-           {MP : map.map K V}
-           (f : K -> V -> A -> ST S A)
-           (p : @map.rep _ _ MP) a : ST S A :=
-  fun g =>
-    map.fold
-      (fun '(g, a) k v => f k v a g)
-      (g, a) p.
-
-Definition map_Miter {S K V}
-           {MP : map.map K V}
-           (f : K -> V -> ST S unit)
-           (p : @map.rep _ _ MP) : ST S unit :=
-  map_Mfold (fun k v _ => f k v) p tt.
-
-(*TODO: double check this is the right name*)
-(* backtracks the state if ma returns None *)       
-Definition try_with_backtrack {S A B}
-           (ma : ST S (Option A)) : ST S (Option A) :=
-  fun g =>
-    match ma g with
-    | (g', Some a) => (g', Some a)
-    | (_, None) => (g, None)
-    end.
+  (*TODO: use coq-record-update?*)
+  Definition set_class_parents '(MkEClass ns _) ps :=
+    MkEClass ns ps.
 
   
-       
-Section EGraphOps.
+  Section EGraphOps.
+    Import StateMonad.
 
-  Local Notation "'ST'" := (ST egraph).
+    Local Notation "'ST'" := (ST egraph).
 
+    Definition find a : ST idx :=
+      fun '(MkEGraph ctx U M H W) =>
+        let (U, i) := UnionFind.find U a in
+        (MkEGraph ctx U M H W,i).
 
-  Definition find a : ST int :=
-    fun '(MkEGraph U M H W) =>
-      let (U, i) := UF.find U a in
-      (MkEGraph U M H W,i).
+    Definition alloc : ST idx :=
+      fun '(MkEGraph ctx U M H W) =>
+        let (U, i) := UnionFind.alloc U in
+        (MkEGraph ctx U M H W,i).
 
-  Definition alloc : ST int :=
-    fun '(MkEGraph U M H W) =>
-      let (U, i) := UF.M.alloc U in
-      (MkEGraph U M H W,i).
+    Definition hashcons_lookup (n : enode) : ST (option idx) :=
+      fun g =>
+        let mi := map.get g.(hashcons) n in
+        (g, mi).
 
-  Definition hashcons_lookup (n : ENode.t) : ST (option int) :=
-    fun g =>
-      let mi := map.get g.(hashcons) n in
-      (g, mi).
-
-  Definition set_hashcons n i : ST unit :=
-    fun '(MkEGraph U M H W) =>
+    Definition set_hashcons n i : ST unit :=
+    fun '(MkEGraph ctx U M H W) =>
       let H := map.put H n i in
-      (MkEGraph U M H W,tt).
-  
-  Definition remove_hashcons n : ST unit :=
-    fun '(MkEGraph U M H W) =>
-      let H := map.remove H n in
-      (MkEGraph U M H W,tt).
-  
-  Definition set_eclass (i: int) (c : EClass.t) : ST unit :=
-    fun '(MkEGraph U M H W) =>
-      let M := map.put M i c in
-      (MkEGraph U M H W,tt).
+      (MkEGraph ctx U M H W,tt).
+    
+    Definition remove_hashcons n : ST unit :=
+      fun '(MkEGraph ctx U M H W) =>
+        let H := map.remove H n in
+        (MkEGraph ctx U M H W,tt).
+    
+    Definition set_eclass (i: idx) (c : eclass) : ST unit :=
+      fun '(MkEGraph ctx U M H W) =>
+        let M := map.put M i c in
+        (MkEGraph ctx U M H W,tt).
 
-  Definition union_ids a b : ST int :=
-    fun '(MkEGraph U M H W) =>
-      let (U, i) := UF.union U a b in
-      (MkEGraph U M H W, i).
+    Definition union_ids a b : ST idx :=
+      fun '(MkEGraph ctx U M H W) =>
+        let (U, i) := UnionFind.union U a b in
+        (MkEGraph ctx U M H W, i).
 
-  (* return a default value rather than none
+    (* return a default value rather than none
      for ease-of-use
-   *)
-  Definition get_eclass (i : int) : ST EClass.t :=
-    (*TODO: using a meaningless default here.
+     *)
+    Definition get_eclass (i : idx) : ST eclass :=
+      (*TODO: using a meaningless default here.
       Decide if an option is better.
       If I want empty as the default,
       I need to decide that ctx and srt don't matter if empty,
       which seems wrong
+       *)
+      fun g => (g, unwrap_with_default eclass_empty (map.get g.(eclasses) i)).
+
+    Definition add_to_worklist (i : idx) : ST unit :=
+      fun '(MkEGraph ctx U M H W) =>
+        let W := i::W in
+        (MkEGraph ctx U M H W, tt).
+
+    (* Returns the worklist for iteration and removes it from the egraph *)
+    Definition pull_worklist : ST (list idx) :=
+      fun '(MkEGraph ctx U M H W) =>
+        (MkEGraph ctx U M H [], W).
+
+    
+    (* Returns the egraph's context *)
+    Definition get_ectx : ST (named_list idx) :=
+      fun g => (g, g.(ectx)).
+    
+    Definition is_worklist_empty : ST bool :=
+      fun g => (g, match g.(worklist) with [] => true | _ => false end).    
+
+    (*adds (n,p) as a parent to i*)
+    Definition add_parent n p i : ST unit :=
+      @! let ci <- get_eclass i in
+         (set_eclass i (eclass_add_parent ci (n,p))).
+    
+    Definition canonicalize n : ST enode :=
+      match n with     
+      | con_node name args =>
+          @! let args <- list_Mmap find args in       
+             ret con_node name args
+      | var_node x =>
+          @! ret var_node x
+      end.
+
+    
+    Definition eqb_ids a b : ST bool :=
+      @! let fa <- (find a) in
+         let fb <- (find b) in
+         ret eqb fa fb.
+
+    
+    Definition lookup n : ST (option idx) :=
+      @! let n <- canonicalize n in
+         (hashcons_lookup n).
+
+    Definition add_parent_to_children n i : ST unit :=
+      match n with
+      | con_node name args =>
+          @! let args <- list_Miter (add_parent n i) args in
+             ret tt
+      | var_node x => @! ret tt
+      end.
+
+    (*
+      Adds a node to the egraph without checking whether it is valid in the language
      *)
-    fun g => (g, unwrap_with_default (EClass.empty 0 0) (map.get g.(eclass_map) i)).
+    Definition add_node_unchecked (n : enode) : ST idx :=
+      @! let mn <- lookup n in
+         match mn with
+         | Some i => @! ret i
+         | None => 
+             @! let i <- alloc in
+                let tt <- set_eclass i (eclass_singleton n) in
+                let tt <- add_parent_to_children n i in
+                let tt <- set_hashcons n i in
+                ret i
+         end.
 
-  Definition add_to_worklist (i : int) : ST unit :=
-    fun '(MkEGraph U M H W) =>
-      let W := i::W in
-      (MkEGraph U M H W, tt).
 
-  (* Returns the worklist for iteration and removes it from the egraph *)
-  Definition pull_worklist : ST (list int) :=
-    fun '(MkEGraph U M H W) =>
-      (MkEGraph U M H [], W).
-  
-  Definition is_worklist_empty : ST bool :=
-    fun g => (g, match g.(worklist) with [] => true | _ => false end).    
+    Context {idx_set : set idx}
+            {eqn_set : set (idx*idx)}.
+    
+    Section WithLang.
 
-  (*adds (n,p) as a parent to i*)
-  Definition add_parent n p i : ST unit :=
-    do let ci : EClass.t <- get_eclass i in
-       (set_eclass i (EClass.add_parent ci (n,p))).
-       
-  Definition canonicalize n : ST ENode.t :=
-    match n with
-    | ctx_empty_node => do ret ctx_empty_node
-    | ctx_cons_node n x srt tl =>
-      do let srt <- find srt in
-         let tl <- find tl in
-         ret ctx_cons_node n x srt tl      
-    | con_node name args =>
-      do let args <- list_Mmap find args in       
-         ret con_node name args     
-    | scon_node name args =>
-      do let args <- list_Mmap find args in       
-         ret scon_node name args
-    | var_node x =>
-      do ret var_node x
-    end.
+      Context (l : lang).
 
-         
-  Definition eqb_ids a b : ST bool :=
-    do let fa <- (find a) in
-       let fb <- (find b) in
-       ret eqb fa fb.
+      
+      (* TODO: add union to interface *)
+      Axiom union : forall {A} {s : set A}, s -> s -> s.
 
-       
-  Definition lookup n : ST (option int) :=
-    do let n <- canonicalize n in
-       (hashcons_lookup n).
+      
+      Section Inner.
+        Context (add_sort' : named_list idx -> sort -> ST (option (idx * eqn_set))).
+        
+        (*  sub is a map from vars to ids with the egraph's ctx as its domain.
+            We need this argument for processing sorts from the language
+         *)
+        Context (sub : named_list idx).
 
-  Definition add_parent_to_children n i : ST unit :=
-    match n with
-    | ctx_empty_node => do ret tt
-    | ctx_cons_node _ x srt tl =>
-      do let tt <- add_parent n i srt in
-         let tt <- add_parent n i tl in
-         ret tt     
-    | con_node name args =>
-      do let args <- list_Miter (add_parent n i) args in
-         ret tt
-    | scon_node name args =>
-      do let args <- list_Miter (add_parent n i) args in
-         ret tt
-    | var_node x => do ret tt
-    end.
+        (* breaks the term down into nodes, computes their sorts,
+         and adds them to the egraph.
+         Returns the top-level node's id and a set of all sort ids
+         that must be equated for the added term to typecheck.
+         Using a set takes advantage of subterm duplicaton to reduce
+         the number of generated goals.
 
-  (* Does not check that the ctx and srt are correct if n already exists
-     TODO: generalize this and 2 sim. fns?
-   *)
-  Definition add_term (n : ENode.t) (ctx srt : int) : ST int :=
-    do let mn <- lookup n in
-       match mn with
-       | Some i => do ret i
-       | None => 
-         do let i <- alloc in
-            let tt <- set_eclass i (EClass.singleton n ctx srt) in
-            let tt <- add_parent_to_children n i in
-            let tt <- add_parent n i srt in
-            let tt <- add_parent n i ctx in
-            let tt <- set_hashcons n i in
-            ret i
-            end.
+         Invariants:
+         If this returns Some v, then:
+         - The added term is well-scoped with respect to the egraph's context
+         - The added term's constructors are all term constructors of the language
+         - All constructors are used with the appropriate arity
 
-  
-  Definition add_ctx (n : ENode.t) : ST int :=
-    do let mn <- lookup n in
-       match mn with
-       | Some i => do ret i
-       | None => 
-         do let i <- alloc in
-            let tt <- set_eclass i (EClass.singleton n 0 0) in
-            let tt <- add_parent_to_children n i in
-            let tt <- set_hashcons n i in
-            ret i
-            end.
+         Thus, if for all (i1, i2) in the eqn_set we have find i1 = find i2,
+         then the added term is well-typed.
+         *)
+
+        (*TODO:
+          machinery for monad transformers
+         *)
+        
+        (*TODO: move to Monad once tested *)
+        Notation "'let' p <?- e 'in' b" :=
+          (Mbind (fun x => match x with p => b | _ => default end) e)
+            (in custom monadic_do at level 200, left associativity, p pattern at level 0, e constr, b custom monadic_do).
+        
+        Fixpoint add_term' (e : term)
+          : ST (option (idx * eqn_set)) :=
+          match e with
+          | var x =>
+              @! let i <- @! ret named_list_lookup_err sub x in
+                 ret (i, map.empty)      
+          | con n s =>
+              @! let term_rule c _ t <?- @!ret named_list_lookup_err l n in
+                 let (s_ids, ids) <- Mfmap Some (add_args s c) in
+                 let ids' := fold_left add_elt s_ids ids in
+                 let (t_id, srt_ids) <- add_sort' (with_names_from c s_ids) t in
+                 let i <- Mfmap Some (add_node_unchecked
+                                        (con_node n (t_id::s_ids))) in
+                 ret (i, union ids' srt_ids)
+          end
+        with add_args (s : list term) c : ST (option (list idx * idx_set)) :=
+               (*TODO: use a for/map notation for this?*)
+               match s with
+               | [] => @! ret ([], map.empty)
+               | e::s =>
+                   @! let (s', ids) <- add_args s in
+                      let i <- add_term e in
+                      foo
+               | _ , _ => @! ret None (*return none? *)
+               end.
+
+    (*
+      Notes about the safety of adding unchecked nodes:
+      - If the node is wf, then it can be kept as-added
+        + Specifically, it can keep its sort since by proving it wf,
+          the egraph will unify its written sort with the other side of any
+          conversion in the wfness proof
+      - If the node is equated with another node, that means they have the same sort
+      Hope: If the node is not wf, then it cannot be equated with a wf node
+
+      If we take this as true, then consider the following algorithm:
+      - add all nodes/terms unchecked
+      - record (TODO: how) all equations that must be proven
+      - iterate to saturation (or step bound)
+      - check that all equations satisfy reflexivity
+     *)
+
+    
+            Fail.
+    (*
+      This datatype helps with terminaton arguments.
+      TODO: fuse generation and consumption?
+     *)
+    Unset Elimination Schemes.
+    Inductive sorted_term : Type :=
+    (* variable name *)
+    | sd_var : idx -> sorted_sort -> sorted_term
+    (* Rule label, list of subterms*)
+    | sd_con : idx -> list sorted_term -> sorted_sort -> sorted_term
+    with sorted_sort : Type := sd_scon : idx -> list sorted_term -> sorted_sort.
+    Set Elimination Schemes.
+
+    (*    
+    Fixpoint lookup_term_with_subst s e : ST (option 
+    Definition lookup_sort_with_subst s t
+     *)
+
+    Section WithChecking.
+
+      Context (l : lang).
+
+      (* Annotate all of the sorts indicated by the language,
+         regardless of whether they line up.
+       *)
+      Fixpoint to_sorted_term (c : named_list sorted_sort) (e : term) :=
+        match e with
+        | Term.var x => sd_var x (named_list_lookup default c x)
+        | Term.con n l =>
+            let t := match named_list_lookup default l n with
+                     | term_rule c' _ t =>
+                         (*TODO: here is the tricky bit of the process*)
+                         to_sorted_sort t
+                     | _ => default
+                     end in
+            sd_con n (map (to_sorted_term c) l) t
+        end.
+
+
+      Fixpoint check_node_arguments (c : ctx) (l : list idx) : ST bool :=
+        match c, l with
+        | [], [] => @! ret true
+        | [], _ => @! ret false
+        | _, [] => @! ret false
+        | (_,t)::c', i::l' =>
+            (*TODO: lookup doesn't suffice; have to add, run saturation? *)
+            @! let Some i' <- lookup_sort_with_subst (with_names_from c' l') t in
+               if eqb i i' then (check_node_arguments c' l') else ret false
+        end.
+      
+      (*
+      checks if a given node is valid in the language,
+      assuming every node in the egraph is valid.
+      Has no effect if the node is invalid.      
+       *)
+      Definition check_sort_node (n : enode) : ST bool :=
+        match n with
+        | var_node x => @! ret None 
+        | con_node n l =>
+            match named_list_lookup l n with
+            | Some (sort_rule c _) => @! ret check_node_arguments c l
+            | None => @! ret false
+            end
+        end.
+      
+                    (*
+                      For a in args, (x,t) in c:
+                          assert (typeof a = t)
+                          
+                      TODO: expects l to be 1 layer deep like nodes;
+                      that is, c should be a named list of idxs
+                     *)
             
-  Definition add_sort (n : ENode.t) ctx : ST int :=
-    do let mn <- lookup n in
-       match mn with
-       | Some i => do ret i
-       | None => 
-         do let i <- alloc in
-            let tt <- set_eclass i (EClass.singleton n ctx 0) in
-            let tt <- add_parent_to_children n i in
-            let tt <- add_parent n i ctx in
-            let tt <- set_hashcons n i in
-            ret i
-            end.
+            
+      (*
+        Like add_sort_node for terms, but also returns the sort of the term
+       *)
+      Definition add_term_node (n : enode) : ST (option (idx (*term*)* idx(*sort*))) :=
+        match n with
+        | var x =>
+            (*TODO: mediate between sorts in ctx and idxs; should they be in the graph?*)
+            @! _ <- nth 
+        | con_node n (srt::args) =>
+        | _ => @! ret None
+      
+    
+    Fail.
 
-  Definition merge (a b : int) : ST int :=
-    do let ca <- find a in
-       let cb <- find b in
-       if eqb ca cb
-       then ret ca
-       else let i <- union_ids a b in
-            let tt <- add_to_worklist i in
-            ret i.
+    (* adds node n at sort srt
+     *)
+    Definition add_term_node (n : enode) (srt : idx) : ST (option idx) :=
+      @! let mn <- lookup n in
+         match mn with
+         | Some i =>
+             @! 
+         | None => 
+             @! let i <- alloc in
+                let tt <- set_eclass i (eclass_singleton n srt) in
+                let tt <- add_parent_to_children n i in
+                (*TODO: should the sort be a parent?
+                  would make more sense to include it in 'get_parents'
+                  rather than saving it twice.
+                  Note that this might interact with the bogus value for sort nodes
+                 *)
+                let tt <- add_parent n i srt in
+                let tt <- set_hashcons n i in
+                ret i
+         end.
+    
+    Definition add_sort_node (n : enode) : ST idx :=
+      @! let mn <- lookup n in
+         match mn with
+         | Some i => @! ret i
+         | None => 
+             @! let i <- alloc in
+                let tt <- set_eclass i (eclass_singleton n zero) in
+                let tt <- add_parent_to_children n i in
+                let tt <- set_hashcons n i in
+                ret i
+         end.
 
-       (*TODO: put in  Monad.v*)
-       Definition seq {M} `{Monad M} {A B} (mu : M A) (ma : M B) : M B :=
-         Mbind (fun _ => ma) mu.
+    Definition merge (a b : idx) : ST idx :=
+      @! let ca <- find a in
+         let cb <- find b in
+         if eqb ca cb
+         then ret ca
+         else let i <- union_ids a b in
+              let tt <- add_to_worklist i in
+              ret i.
 
-       Notation "e1 ; e2" :=
-         (seq e1 e2)
-           (in custom monadic_do at level 100, left associativity,
-               e1 custom monadic_do,
-               e2 custom monadic_do).
 
-
-       (*TODO: generalize, put in Monad.v*)
-       Notation "'for' kp vp 'from' m 'in' b" :=
-         (*TODO: remove need for explicit instance*)
-         (map_Miter (MP:=hashcons_ty) (fun kp vp => b) m)                       
-           (in custom monadic_do at level 200, left associativity,
-               kp pattern at level 0,
-               vp pattern at level 0,
-               m constr, b custom monadic_do).
-       
-       Notation "'for/fold' kp vp 'from' m [[ acc := a ]] 'in' b" :=
-         (*TODO: remove need for explicit instance*)
-         (map_Mfold (MP:=hashcons_ty) (fun kp vp acc => b) a m)                       
-           (in custom monadic_do at level 200, left associativity,
-               kp pattern at level 0,
-               vp pattern at level 0,
-               acc pattern at level 0,
-               m constr, b custom monadic_do).
-
-  (*TODO: use coq-record-update?*)
-  Definition set_class_parents '(MkEClass ns _ ntx nsrt) ps :=
-    MkEClass ns ps ntx nsrt.
-
-  (*TODO: think about parents wrt srt, ctx
-    if c |- e : t, then e is a parent of c, t
+    (*TODO: think about parents wrt srt, ctx
+    if c |- e : t, then e is a parent of t
     need to set those somewhere
-   *)
-  Definition repair i : ST unit :=
-    do let c <- get_eclass i in
-       let tt <- do for pn pi from c.(parents) in
-                 let tt <- remove_hashcons pn in
-                 let pn <- canonicalize pn in
-                 let ci <- find pi in
-                 (set_hashcons pn ci) in
-       let new_parents <- do for/fold pn pi from c.(parents)
-                                [[new_parents := (map.empty : hashcons_ty)]] in
-                          let pn <- canonicalize pn in
-                          match map.get new_parents pn : option int return ST map.rep with
-                          | Some np => seq (merge pi np) (do ret new_parents)
-                          | None =>
-                            do let ci <- find pi in
-                               ret (map.put new_parents pn ci)
-                          end in
-       (set_eclass i (set_class_parents c new_parents)).
+     *)
+    Definition repair (i : idx) : ST unit :=
+      @! let c <- get_eclass i in
+         let tt <- @! for pn pi from c.(parents) in
+         let tt <- remove_hashcons pn in
+         let pn <- canonicalize pn in
+         let ci <- find pi in
+         (set_hashcons pn ci) in
+           let new_parents <-
+                 @! for/fold pn pi
+                    from c.(parents)
+                             [[new_parents := (map.empty : node_map)]] in
+           let pn <- canonicalize pn in
+           match map.get new_parents pn : option idx return ST map.rep with
+             
+           | Some np => Mseq (merge pi np) (@! ret new_parents)
+           | None =>
+               @! let ci <- find pi in
+                  ret (map.put new_parents pn ci)
+           end in
+             (set_eclass i (set_class_parents c new_parents)).
 
-  Definition rebuild_aux : N -> ST unit :=
-    N.recursion
-      (Mret tt)
-      (fun _ rec =>
-         do let (is_empty : bool) <- is_worklist_empty in
-            if is_empty then ret tt
-            else
-              let tt <- rec in
-              let W <- pull_worklist in
-              (*TODO: should worklist and/or cW be a set? Egg has a dedup step.
-                For now we are not deduplicating here, but we probably should at some point
-               *)
-              let cW <- list_Mmap find W in
-              (list_Miter repair cW)).
-                               
-  (* TODO: need to track  I = ~=\=_node to use as fuel
-   *)
-  Definition rebuild : ST unit :=
-    do let incong_bound := 100 in
-       (rebuild_aux 100).
+    Definition rebuild_aux : N -> ST unit :=
+      N.recursion
+        (Mret tt)
+        (fun _ rec =>
+           @! let (is_empty : bool) <- is_worklist_empty in
+              if is_empty then ret tt
+              else
+                let tt <- rec in
+                let W <- pull_worklist in
+                (*TODO: should worklist and/or cW be a set? Egg has a dedup step.
+                For now we are not deduplicating here, but we probably should at some poidx
+                 *)
+                let cW <- list_Mmap find W in
+                (list_Miter repair cW)).
+    
+    (* TODO: need to track  I = ~=\=_node to use as fuel
+     *)
+    Definition rebuild : ST unit :=
+      @! let incong_bound := 100 in
+         (rebuild_aux 100).
+
+    Context {arg_map : map.map idx idx}.
+    
+    (* Higher-level term operations*)
+
+    (* Concept: add all terms at once, good or not,
+       and equate them incrementally.
+       In proofs, need to keep track of which ids are dangerous.
+       Allows us to write the full tree, then do reads for the sort equations
+     *)
+    
+
+
+      Fail.
 
   (* TODO: is it worth using a more efficient structure?
      If we assume that the max length is ~10, maybe not
    *)
-  Definition esubst := list (int*int).
-  Definition match_result := list (esubst * EClass.t).
-
+  Definition esubst := list (idx*idx).
+  Definition match_result := list (esubst * eclass).
   
 
   (*Used as an intermediate form in equality saturation *)
   Unset Elimination Schemes.
-  (*TODO: parameterize; replace int with Idx.t*)
+  (*TODO: parameterize; replace idx with Idx.t*)
   Inductive eterm : Set :=
   (* variable name *)
-  | evar : int -> eterm
+  | evar : idx -> eterm
   (* Rule label, list of subterms*)
-  | econ : int -> list eterm -> eterm
+  | econ : idx -> list eterm -> eterm
+  (* new constructor: *)
   (* reference to an existing node in the egraph *)
-  | eref : int -> eterm.
+  | eref : idx -> eterm.
   Set Elimination Schemes.
 
 
   (* TODO: zero is a questionable default unless I implement null idea*)
-  Fixpoint esubst_lookup (s : esubst) (n : int) : int :=
+  Fixpoidx esubst_lookup (s : esubst) (n : idx) : idx :=
     match s with
-    | [] => 0%int63
+    | [] => 0%idx63
     | (s', v)::l' =>
       if eqb n s' then v else esubst_lookup l' n
     end.
 
   Arguments esubst_lookup !s n/.
 
-  Import Int63Term.
+  Import Idx63Term.
   (*TODO: take in an actual map for constr_map?*)
   Fixpoint to_eterm (e : term) : eterm :=
     match e with
@@ -690,12 +553,12 @@ Section EGraphOps.
   Arguments eterm_subst s !e /.
 
   
-  Definition lookup_sort (tm : int) : ST int :=
-    do let c <- get_eclass tm in
+  Definition lookup_sort (tm : idx) : ST idx :=
+    @! let c <- get_eclass tm in
        ret c.(esrt).
        
-  Definition lookup_ctx (tm : int) : ST int :=
-    do let c <- get_eclass tm in
+  Definition lookup_ctx (tm : int) : ST idx :=
+    @! let c <- get_eclass tm in
        ret c.(ectx).
 
 
@@ -703,22 +566,22 @@ Section EGraphOps.
             (rec : ctx_idx -> var_idx -> ST (option srt_idx))
             (ctx : ctx_idx)
             (x : var_idx) : ST (option srt_idx) :=
-    do let c <- get_eclass ctx in
+    @! let c <- get_eclass ctx in
        match NodeSets.choose c.(nodes) with
        | Some (ctx_cons_node _ x' srt tl) =>
-         if eqb x x' then do ret Some srt
+         if eqb x x' then @! ret Some srt
          else rec tl x
-       | _ => do ret None
+       | _ => @! ret None
        end.
 
   (*TODO: try to collapse 2 defs*)
-  Definition lookup_sort_in_ctx (ctx x : int) : ST (option srt_idx) :=
-    do let c <- get_eclass ctx in
+  Definition lookup_sort_in_ctx (ctx x : idx) : ST (option srt_idx) :=
+    @! let c <- get_eclass ctx in
        match NodeSets.choose c.(nodes) with
        | Some (ctx_cons_node n x' srt tl) =>
-         if eqb x x' then do ret Some srt
-         else N.recursion (fun _ _ => do ret None) (fun _ => lookup_sort_in_ctx') n tl x
-       | _ => do ret None
+         if eqb x x' then @! ret Some srt
+         else N.recursion (fun _ _ => @! ret None) (fun _ => lookup_sort_in_ctx') n tl x
+       | _ => @! ret None
        end.       
 
   (*TODO: want this to be fast.
@@ -735,16 +598,16 @@ Section EGraphOps.
   (* assumes that the context and sort have already been added *)
   (* TODO: think about read/write separation & invariants *)
   (* TODO: needs lang as input to generate the sort *)
-  Fixpoint add_eterm_no_check lang (ctx (*srt*): int) (e : eterm) : ST (option int) :=
+  Fixpoint add_eterm_no_check lang (ctx (*srt*): idx) (e : eterm) : ST (option idx) :=
     match e with
     | evar x =>
-      do let srt <- lookup_sort_in_ctx ctx x in
+      @! let srt <- lookup_sort_in_ctx ctx x in
          (add_term (var_node x) ctx srt)
     | econ n s =>
       (*TODO: generalize list_Mmap to composition of ST and option.
         Requires monad transformers to be nice
        *)
-      do let margs <- list_Mmap add_eterm s in
+      @! let margs <- list_Mmap add_eterm s in
          let srt <- 
          match List.option_all margs with
          | Some args =>
@@ -753,7 +616,7 @@ Section EGraphOps.
            (add_term (con_node n args) ctx srt)
          | None => None
          end
-    | eref i => do ret i
+    | eref i => @! ret i
    end.
 
                                                                              
@@ -765,10 +628,10 @@ Section EGraphOps.
      ^ TODO: do this
    *)
   (*TODO: does this need to take an eterm? *)
-  Fixpoint check_and_add_eterm (ctx (*srt*): int) (e : eterm) : ST (option int) :=
+  Fixpoint check_and_add_eterm (ctx (*srt*): idx) (e : eterm) : ST (option int) :=
     match e with
     | evar x =>
-      do let srt <- lookup_sort_in_ctx ctx x in
+      @! let srt <- lookup_sort_in_ctx ctx x in
          (add_term (var_node x) ctx srt)
       (*TODO: need to look up sort
        and check, if srt is provided*)
@@ -777,7 +640,7 @@ Section EGraphOps.
       (*TODO: generalize list_Mmap to composition of ST and option.
         Requires monad transformers to be nice
        *)
-      do let margs <- list_Mmap add_eterm s in
+      @! let margs <- list_Mmap add_eterm s in
          match List.option_all margs with
          | Some args =>
            (*TODO: check wfness of top-level constructor here*)
@@ -799,7 +662,7 @@ Section EGraphOps.
     match e with
     | var x => TODO
     | con n s =>
-      do let ematch_s <- list_Mmap ematch s in
+      @! let ematch_s <- list_Mmap ematch s in
          TODO
          end.
 
@@ -812,16 +675,16 @@ Section EGraphOps.
 
             w/ this API, ctx nodes seem reasonable
           *)
-         Parameter add_and_check_wf_term : lang -> ctx -> term -> ST (option int).
-         Parameter add_and_check_wf_sort : lang -> ctx -> term -> ST (option int).
-         Parameter get_term : int -> ST (option term).
-         Parameter get_ctx_of_term : int -> ST (option ctx).
-         Parameter get_sort_of_term : int -> ST (option sort).
-         Parameter get_sort : int -> ST (option sort).
+         Parameter add_and_check_wf_term : lang -> ctx -> term -> ST (option idx).
+         Parameter add_and_check_wf_sort : lang -> ctx -> term -> ST (option idx).
+         Parameter get_term : idx -> ST (option term).
+         Parameter get_ctx_of_term : idx -> ST (option ctx).
+         Parameter get_sort_of_term : idx -> ST (option sort).
+         Parameter get_sort : idx -> ST (option sort).
 
          (* one of these two *)
          Parameter saturate : lang -> ST unit.
-         Parameter saturate_until_eq : lang -> int -> int -> ST bool.
+         Parameter saturate_until_eq : lang -> idx -> idx -> ST bool.
 
          (* assumes saturation *)
          Definition compare_eq l i1 i2 : ST bool :=
@@ -857,3 +720,5 @@ Definition ematch_term_sound g : Prop :=
 (*corollary: 
   egraph_sound_in_lang g l ->
   wf_subst l c' s c *)
+
+*)
