src/Utils/ExtraMaps.v
@@ -1,0 +1,56 @@
+From coqutil Require Import Map.Interface.
+(*
+TODO: implement map with tries?
+Require Import Tries.Canonical.
+
+TODO: implement map Int63 with ArrayList?
+*)
+
+Module IntersectableMap.
+
+  Class intersectable_map (K V : Type) :=
+    {
+      map :> map.map K V;
+      intersection : map -> map -> map
+    }.
+  Arguments intersectable_map : clear implicits.
+  Local Coercion map : intersectable_map >-> map.map.
+  
+  Class ok {K V} (imap : intersectable_map K V) :=
+    {
+      map_ok :> map.ok imap;
+      get_intersect_same : forall (m1 m2 : imap) k,
+        map.get m1 k = map.get m2 k ->
+        map.get (intersection m1 m2) k = map.get m1 k;
+      get_intersect_diff : forall (m1 m2 : imap) k,
+        ~ (map.get m1 k = map.get m2 k) ->
+        map.get (intersection m1 m2) k = None;
+    }.
+
+End IntersectableMap.
+Global Coercion IntersectableMap.map : IntersectableMap.intersectable_map >-> map.map.
+Notation intersection := IntersectableMap.intersection.
+
+
+Module Sets.
+  Section __.
+    Context {A:Type}.
+
+    Notation set := (IntersectableMap.intersectable_map A unit).
+
+    Context {set_instance : set}.
+
+    Local Hint Mode map.map - - : typeclass_instances.  
+
+    Definition member s (a : A) :=
+      if map.get s a then true else false.
+
+    Definition add_elt s (a : A) :=
+      map.put s a tt.
+
+  End __.
+
+  Global Notation set A := (IntersectableMap.intersectable_map A unit).
+  
+End Sets.
+
